spot/GC.SPOT.HeapExpansion.fst
@@ -2085,6 +2085,8 @@ let spot_chunked_cheney_promote_after_minor_promotion_head_preflight
            r.capacity_major_out r.capacity_fp_out r.capacity_fuel_out /\
          CheneyPreservation.chunked_fwd_targets_above_minor res.fwd_map /\
          CheneyPreservation.chunked_fwd_targets_valid_addr res.fwd_map /\
+         CheneyPreservation.chunked_fwd_noninfix_targets_in_major
+           minor res.fwd_map res.major_final /\
          (forall (x:U64.t).
            Seq.mem x (minor_reachable minor roots) /\
            minor_wosize minor x > 0 ==>
@@ -3832,6 +3834,8 @@ let spot_chunked_cheney_collect_after_minor_promotion_head_preflight
          collect.cmc_fwd == prom.fwd_map /\
          CheneyPreservation.chunked_fwd_targets_above_minor collect.cmc_fwd /\
          CheneyPreservation.chunked_fwd_targets_valid_addr collect.cmc_fwd /\
+         CheneyPreservation.chunked_fwd_noninfix_targets_in_major
+           minor collect.cmc_fwd collect.cmc_major /\
          GenInv.chunked_major_alloc_shape
            collect.cmc_major collect.cmc_fp r.capacity_fuel_out /\
          SpecMajorAlloc.major_fl_chain_terminates
@@ -4002,6 +4006,8 @@ let spot_chunked_cheney_gc_correct_after_preflight
          collect.cmc_fwd == prom.fwd_map /\
          CheneyPreservation.chunked_fwd_targets_above_minor collect.cmc_fwd /\
          CheneyPreservation.chunked_fwd_targets_valid_addr collect.cmc_fwd /\
+         CheneyPreservation.chunked_fwd_noninfix_targets_in_major
+           minor collect.cmc_fwd collect.cmc_major /\
          GenInv.chunked_major_alloc_shape
            collect.cmc_major collect.cmc_fp r.capacity_fuel_out /\
          SpecMajorAlloc.major_fl_chain_terminates
@@ -4049,6 +4055,92 @@ let spot_chunked_cheney_gc_correct_after_preflight
   =
   CheneyCorrectness.chunked_cheney_gc_correct_after_preflight
     minor major fp roots alloc_fuel fresh
+
+let spot_chunked_cheney_gc_correct_after_preflight_forwarded_minor_object_in_major
+  (minor: minor_state) (major: MH.major_heap) (fp: U64.t)
+  (roots: Seq.seq U64.t) (alloc_fuel: nat) (fresh: MH.heap_chunk)
+  (x: U64.t)
+  : Lemma
+      (requires
+        minor_wf minor /\
+        alloc_fuel > 1 /\
+        GenInv.chunked_collection_heap_shape minor major fp alloc_fuel /\
+        SpecMajorAlloc.major_fl_chain_terminates
+          major fp alloc_fuel = true /\
+        GenInv.chunked_chain_objects_blue major fp alloc_fuel /\
+        (SpecMajorAlloc.major_fl_head_wosize major fp <
+          PromotionDemand.minor_promotion_demand minor + 1 ==>
+          MH.chunk_disjoint_from_all fresh major /\
+          fp <> SpecMajorAlloc.fresh_chunk_object fresh /\
+          U64.v fresh.base >= U64.v zero_addr /\
+          SpecMajorAlloc.fresh_chunk_wosize fresh >=
+            PromotionDemand.minor_promotion_demand minor + 1 /\
+          CG.chunked_all_major_object_expansion_safe
+            major fresh (MH.major_objects major) 0) /\
+        Seq.mem x (minor_objects minor) /\
+        (let needed = PromotionDemand.minor_promotion_demand minor + 1 in
+         let r =
+          SpecMajorAlloc.ensure_major_head_capacity_spec
+            major fp alloc_fuel needed fresh in
+         let collect =
+          ChunkedCheney.chunked_cheney_collect_spec
+            minor r.capacity_major_out r.capacity_fp_out roots
+            r.capacity_fuel_out in
+         collect.cmc_fwd x <> 0UL))
+      (ensures
+        (let needed = PromotionDemand.minor_promotion_demand minor + 1 in
+         let r =
+          SpecMajorAlloc.ensure_major_head_capacity_spec
+            major fp alloc_fuel needed fresh in
+         let collect =
+          ChunkedCheney.chunked_cheney_collect_spec
+            minor r.capacity_major_out r.capacity_fp_out roots
+            r.capacity_fuel_out in
+         is_val_addr (collect.cmc_fwd x) /\
+         Seq.mem ((collect.cmc_fwd x) <: obj_addr)
+          (MH.major_objects collect.cmc_major)))
+  =
+  CheneyCorrectness.chunked_cheney_gc_correct_after_preflight_forwarded_minor_object_in_major
+    minor major fp roots alloc_fuel fresh x
+
+let spot_chunked_cheney_gc_correct_after_preflight_reachable_forwarding_target_in_major
+  (minor: minor_state) (major: MH.major_heap) (fp: U64.t)
+  (roots: Seq.seq U64.t) (alloc_fuel: nat) (fresh: MH.heap_chunk)
+  (x: U64.t)
+  : Lemma
+      (requires
+        minor_wf minor /\
+        alloc_fuel > 1 /\
+        GenInv.chunked_collection_heap_shape minor major fp alloc_fuel /\
+        SpecMajorAlloc.major_fl_chain_terminates
+          major fp alloc_fuel = true /\
+        GenInv.chunked_chain_objects_blue major fp alloc_fuel /\
+        (SpecMajorAlloc.major_fl_head_wosize major fp <
+          PromotionDemand.minor_promotion_demand minor + 1 ==>
+          MH.chunk_disjoint_from_all fresh major /\
+          fp <> SpecMajorAlloc.fresh_chunk_object fresh /\
+          U64.v fresh.base >= U64.v zero_addr /\
+          SpecMajorAlloc.fresh_chunk_wosize fresh >=
+            PromotionDemand.minor_promotion_demand minor + 1 /\
+          CG.chunked_all_major_object_expansion_safe
+            major fresh (MH.major_objects major) 0) /\
+        Seq.mem x (minor_reachable minor roots) /\
+        minor_wosize minor x > 0)
+      (ensures
+        (let needed = PromotionDemand.minor_promotion_demand minor + 1 in
+         let r =
+          SpecMajorAlloc.ensure_major_head_capacity_spec
+            major fp alloc_fuel needed fresh in
+         let collect =
+          ChunkedCheney.chunked_cheney_collect_spec
+            minor r.capacity_major_out r.capacity_fp_out roots
+            r.capacity_fuel_out in
+         is_val_addr (collect.cmc_fwd x) /\
+         Seq.mem ((collect.cmc_fwd x) <: obj_addr)
+          (MH.major_objects collect.cmc_major)))
+  =
+  CheneyCorrectness.chunked_cheney_gc_correct_after_preflight_reachable_forwarding_target_in_major
+    minor major fp roots alloc_fuel fresh x
 
 let spot_chunked_update_forwarded_minor_field_edge
   (minor: minor_state) (mh: MH.major_heap) (fwd: forwarding_map)
@@ -4260,6 +4352,55 @@ let spot_chunked_forward_fields_preserved_forwarded_minor_field_edge
   =
   CheneyCorrectness.chunked_forward_fields_preserved_forwarded_minor_field_edge
     minor cs parent idx wosize alloc_fuel src expected hdr j field_addr old
+
+let spot_chunked_forward_fields_preserved_minor_object_field_edge
+  (minor: minor_state) (cs: ChunkedCheney.chunked_cheney_state)
+  (parent: U64.t) (idx wosize alloc_fuel: nat)
+  (src: obj_addr) (hdr: U64.t) (j: nat)
+  (field_addr: hp_addr) (old: U64.t)
+  : Lemma
+      (requires
+        minor_wf minor /\
+        alloc_fuel > 1 /\
+        GenInv.chunked_major_alloc_shape
+          cs.ccs_major cs.ccs_fp alloc_fuel /\
+        SpecMajorAlloc.major_fl_chain_terminates
+          cs.ccs_major cs.ccs_fp alloc_fuel = true /\
+        GenInv.chunked_chain_objects_blue
+          cs.ccs_major cs.ccs_fp alloc_fuel /\
+        CheneyPreservation.chunked_cheney_forward_fields_split_ready
+          minor cs parent idx wosize alloc_fuel /\
+        Seq.mem src (MH.major_objects cs.ccs_major) /\
+        MH.read_word_in_major cs.ccs_major (hd_address src) == Some hdr /\
+        Obj.getColor hdr <> GC.Lib.Header.Blue /\
+        U64.v (Obj.getTag hdr) < U64.v Obj.no_scan_tag /\
+        j < U64.v (Obj.getWosize hdr) /\
+        U64.v field_addr == U64.v src + j * U64.v mword /\
+        CG.chunked_major_field_slot src j == Some field_addr /\
+        MH.read_word_in_major cs.ccs_major field_addr == Some old /\
+        (let cs' =
+          ChunkedCheney.chunked_cheney_forward_fields
+            minor cs parent idx wosize alloc_fuel in
+         let x = to_minor_offset old in
+         CheneyPreservation.chunked_fwd_targets_above_minor cs'.ccs_fwd /\
+         CheneyPreservation.chunked_fwd_noninfix_targets_in_major
+          minor cs'.ccs_fwd cs'.ccs_major /\
+         is_minor_pointer x /\
+         Seq.mem x (minor_objects minor) /\
+         cs'.ccs_fwd x <> 0UL))
+      (ensures
+        (let cs' =
+          ChunkedCheney.chunked_cheney_forward_fields
+            minor cs parent idx wosize alloc_fuel in
+         let x = to_minor_offset old in
+         CG.mem_ce (CG.MajorV src, CG.MajorV (cs'.ccs_fwd x))
+          (CG.build_chunked_combined_graph
+            (minor_reset minor)
+            (ChunkedUpdate.chunked_update_major_pointers
+              cs'.ccs_major cs'.ccs_fwd))))
+  =
+  CheneyCorrectness.chunked_forward_fields_preserved_minor_object_field_edge
+    minor cs parent idx wosize alloc_fuel src hdr j field_addr old
 
 let spot_chunked_cheney_gc_correct_after_preflight_old_major_field_edge
   (minor: minor_state) (major: MH.major_heap) (fp: U64.t)
